forst draft of the basic protocol implementation in F*, still no attacker and lots to do on naming and readability

SAMLProtocol.fst
@@ -1,53 +1,93 @@
 module PROTOCOL
 
-type prin = string
-type samlmessage = string
+type prin
+type samlmessage
 type response
 type dsig
 type resource
+type uri
 
-val requestResource: prin -> unit
-val revcievehttpResponse: prin -> resource
-val sendhttpRedirect: prin -> bytes -> dsig -> string -> unit
+val createAuthnRequest: prin -> prin -> (samlmessage * dsig)
+val createChallenge: prin -> string
+val createSamlResponse: prin -> prin -> (samlmessage * dsig)
+
+val recieveHttpRequest: prin -> uri
+val recieveHttpResponse: prin -> resource
+val recieveAutenticationRequestChallenge: prin -> string
+val recieveAutenticationRequest: prin -> (string * string * string)
+val recieveAutenticationCredentials: prin -> (samlmessage * dsig * string)
 val recievehttpRedirect: prin -> (prin * samlmessage * dsig * string)
-val sendAuthnRequest: prin -> samlmessage -> dsig -> samlmessage -> unit
-val retrieveAutenticationRequestChallenge: prin -> string
+
+val sendRequestResource: prin -> unit
+val sendhttpRedirect: prin -> prin -> samlmessage -> dsig -> string -> unit
+val sendAuthnRequest: prin -> samlmessage -> dsig -> string -> unit
 val sendAutenticationRequest: prin -> string -> string -> string -> unit
+val sendAutenticationChallenge: prin -> string -> unit
 val sendAuthentication: prin -> samlmessage -> string -> unit
+val sendResource: prin -> resource
 
 end (*PROTOCOL*)
 
 module CLIENT
 open PROTOCOL
 
-val client: prin -> user:string -> password:string -> unit
+(*
+- Protocol events
+- Add assumtions
+- Add asserts
+  *)
+
+val client: me:prin -> user:string -> password:string -> unit
 let client sp user password = 
-    let _ = requestResource sp in(*1*)
-    let (idp, authnRequest, sigSP, relayState) = recievehttpRedirect sp in(*2*)
-      sendAuthnRequest idp authnRequest sigSP relayState;(*3*)
-      let challenge = retrieveAutenticationRequestChallenge idp in(*4*)
-        sendAutenticationRequest idp user password challenge; (*5*)
-        let (sp', samlResponse, sigIDP, relayState') = recievehttpRedirect idp in(*6*)
-          sendAuthentication sp' samlResponse relayState'; (*7*)
-          let res = revcievehttpResponse sp' in (*8*)
-          ()
+    let _ = sendRequestResource sp in(*1*)
+      let (idp, authnRequest, sigSP, relayState) = recievehttpRedirect sp in(*2*)
+        sendAuthnRequest idp authnRequest sigSP relayState;(*3*)
+        let challenge = recieveAutenticationRequestChallenge idp in(*4*)
+          sendAutenticationRequest idp user password challenge; (*5*)
+          let (sp', samlResponse, sigIDP, relayState') = recievehttpRedirect idp in(*6*)
+            sendAuthentication sp' samlResponse relayState'; (*7*)
+            let res = recieveHttpResponse sp' in (*8*)
+            ()
 end (*CLIENT*)
 
 
 module SERVICEPROVIDER
 open PROTOCOL
-open CLIENT
 
-(*  val id : string
-  val issueInstant : string
-  val destination : string
-  val issuer : string
-  val condition : string 
-  *)
+(*
+- Protocol events
+- Add assumtions
+- Add asserts
+*)
+
+val serviceprovider: me:prin -> client:prin -> idp:prin -> unit 
+let serviceprovider me client idp = 
+  let reqUri = recieveHttpRequest client in (*1*)
+    let (authnReq, sigSP)  = createAuthnRequest me idp in 
+      sendAuthnRequest client authnReq sigSP "relay"; (*2*)
+      let (sp, samlResponse, sigIDP, relay) = recievehttpRedirect client in (*7*)
+        sendResource client; (*8*)
+        ()
+
 end (* SERVICEPROVIDER *)
 
 module IDENTITYPROVIDER
 open PROTOCOL
 
+(*
+- Protocol events
+- Add assumtions
+- Add asserts
+*)
 
-end
+val identityprovider: me:prin -> client:prin -> sp:prin -> unit
+let identityprovider me client serviceprovider =
+  let (authnReq, sigSP, relay) = recieveAutenticationRequest client in (*3*)
+    let challenge = createChallenge client in
+      sendAutenticationChallenge client challenge; (*4*)
+      let (user,password, challenge') = recieveAutenticationCredentials client in (*5*)
+        let (samlResponse, sigIDP) = createSamlResponse me serviceprovider in 
+          sendhttpRedirect client serviceprovider samlResponse sigIDP; (*6*)
+          ()
+
+end (*IDENTITYPROVIDER*)
